Extracted the general strong simulation adequacy for heap lang

fairness/heap_lang/em_lm.v
@@ -4,7 +4,7 @@ From iris.proofmode Require Import tactics.
 
 
 Definition LM_init_resource `{LM:LiveModel heap_lang Mdl} `{!fairnessGS LM Σ}
-  (s1: fmstate Mdl)
+  (s1: LM)
   (* FR *)
   : iProp Σ :=
   frag_model_is s1 ∗
@@ -15,43 +15,23 @@ Definition init_thread_post `{LM:LiveModel heap_lang M} `{!fairnessGS LM Σ}
   (tid: locale heap_lang): iProp Σ :=
   tid ↦M ∅.
 
-
-Global Instance LM_EM `{LM: LiveModel heap_lang M}: @ExecutionModel LM :=
-  {|
-    em_preGS := fun Σ => fairnessGpreS LM Σ;
-    em_GS := fun Σ => fairnessGS LM Σ;
-    em_Σ := fairnessΣ heap_lang M;
-    em_Σ_subG := fun Σ => @subG_fairnessGpreS _ _ _ LM _ _;
-
-    em_valid_state_evolution_fairness := valid_state_evolution_fairness;
-    em_thread_post Σ := fun {_: fairnessGS LM Σ} (tid: locale heap_lang) (_: val) => tid ↦M ∅;
-    (* TODO: cannot express the msi instantiation this way*)
-    em_msi Σ := fun {_: fairnessGS LM Σ} es δ => model_state_interp es δ;                                                                                    
-    em_init_resource Σ := fun {_: fairnessGS LM Σ} δ => LM_init_resource δ;
-|}.
-
-(* TODO: get rid of it*)
-Global Instance LM_EM_fairPre `{LM: LiveModel heap_lang M}
-                `{hGS: @heapGpreS Σ LM (@LM_EM _ LM)}:
-  fairnessGpreS LM Σ.
-Proof. apply hGS. Defined. 
-
-(* TODO: get rid of it*)
-Global Instance LM_EM_fair `{LM: LiveModel heap_lang M}
-                `{hGS: @heapGS Σ LM (@LM_EM _ LM)}:
-  fairnessGS LM Σ.
-Proof. apply hGS. Defined.
+Definition lm_init `{LM: LiveModel heap_lang M} (δ: mstate LM) :=
+  ls_fuel δ = gset_to_gmap (lm_fl LM δ) (live_roles _ (ls_under δ)) /\
+  ls_mapping δ = gset_to_gmap 0%nat (live_roles _ (ls_under δ)). 
 
 (* TODO: how to make 'heap..' instantiations less wordy? *)
-Lemma init_fairnessGS_LM Σ `(LM:LiveModel heap_lang M)
-  `{hPre: @heapGpreS Σ LM (@LM_EM _ LM)}
-  (s1: M) (e1 : expr):
+(* TODO: how to avoid different instances of EqDec and Cnt? *)
+Lemma init_fairnessGS_LM Σ `{hPre: @fairnessGpreS heap_lang M LM Σ
+                                     Nat.eq_dec nat_countable
+  }
+  (* `(LM:LiveModel heap_lang M)   *)
+  (s1: LM) (e1 : expr) (INIT: lm_init s1):
   ⊢ (|==> ∃ fGS: fairnessGS LM Σ, (* TODO: what is a canonical way of doing it? *)
-       ∀ `{hGS: @heapGS Σ _ (@LM_EM _ LM)},
-         ⌜ hGS.(heap_fairnessGS) = fGS⌝ →
-      LM_init_resource s1 ∗ model_state_interp [e1] (initial_ls s1 0%nat (LM := LM))).
+       (* ∀ `{hGS: @heapGS Σ _ (@LM_EM _ LM)}, *)
+       (*   ⌜ hGS.(heap_fairnessGS) = fGS⌝ → *)
+      LM_init_resource s1 ∗ model_state_interp [e1] s1).
 Proof.
-  iIntros.
+  iIntros. destruct INIT as [FUEL MAP]. 
   iMod (model_state_init s1) as (γmod) "[Hmoda Hmodf]".
   iMod (model_mapping_init s1) as (γmap) "[Hmapa Hmapf]".
   iMod (model_fuel_init s1) as (γfuel) "[Hfuela Hfuelf]".
@@ -59,25 +39,31 @@ Proof.
   (* iMod (model_free_roles_init s1 (FR ∖ live_roles _ s1)) as (γfr) "[HFR Hfr]". *)
   iMod (model_free_roles_init s1 ∅) as (γfr) "[HFR Hfr]".
   iModIntro.
-  iExists ({|
+  iExists ({| 
+              fairness_inG := hPre;
               fairness_model_name := γmod;
               fairness_model_mapping_name := γmap;
               fairness_model_fuel_name := γfuel;
               fairness_model_free_roles_name := γfr;
             |}).
-  iIntros.
 
   iSplitL "Hmodf Hfr Hfuelf Hmapf".
   2: { unfold model_state_interp. simpl. iFrame. 
        iExists {[ 0%nat := (live_roles M s1) ]}, _.
-       iSplitL "Hfuela"; first by rewrite /auth_fuel_is /= fmap_gset_to_gmap //.
+
+       (* iSplitL "Hfuela"; first by rewrite /auth_fuel_is /= fmap_gset_to_gmap //. *)
+       iSplitL "Hfuela".
+       { rewrite /auth_fuel_is /=.
+         rewrite FUEL. rewrite fmap_gset_to_gmap //. } 
+
        iSplitL "Hmapa"; first by rewrite /auth_mapping_is /= map_fmap_singleton //.
        iSplit; first done.
        iSplit; iPureIntro; [|split].
-       - intros ρ tid. rewrite lookup_gset_to_gmap_Some.
+       - intros ρ tid. rewrite MAP. 
+         rewrite lookup_gset_to_gmap_Some.
          setoid_rewrite lookup_singleton_Some. split; naive_solver.
        - intros tid Hlocs. rewrite lookup_singleton_ne //. compute in Hlocs. set_solver.
-       - rewrite dom_gset_to_gmap. set_solver. }
+       - rewrite FUEL. rewrite dom_gset_to_gmap. set_solver. }
 
   rewrite /LM_init_resource.
   rewrite /has_fuels /frag_mapping_is /= map_fmap_singleton.
@@ -101,3 +87,36 @@ Proof.
   iExists _. iFrame. iPureIntro. apply lookup_gset_to_gmap_Some. done.
 Qed.
 
+
+Global Instance LM_EM `{LM: LiveModel heap_lang M}: @ExecutionModel LM.
+refine
+  {|
+    em_preGS := fun Σ => fairnessGpreS LM Σ;
+    em_GS := fun Σ => fairnessGS LM Σ;
+    em_Σ := fairnessΣ heap_lang M;
+    em_Σ_subG := fun Σ => @subG_fairnessGpreS _ _ _ LM _ _;
+
+    em_valid_state_evolution_fairness := valid_state_evolution_fairness;
+    em_thread_post Σ := fun {_: fairnessGS LM Σ} (tid: locale heap_lang) (_: val) => tid ↦M ∅;
+    (* TODO: cannot express the msi instantiation this way*)
+    em_msi Σ := fun {_: fairnessGS LM Σ} es δ => model_state_interp es δ;                                                                                      
+    em_init_state := lm_init;     
+
+    em_init_resource Σ := fun {_: fairnessGS LM Σ} δ => LM_init_resource δ;
+|}.
+intros. iIntros. iMod (init_fairnessGS_LM _ s1 e1) as "[% [? X]]"; [done| ]. 
+iModIntro. iExists _. iFrame.
+Defined. 
+
+(* TODO: get rid of it*)
+Global Instance LM_EM_fairPre `{LM: LiveModel heap_lang M}
+                `{hGS: @heapGpreS Σ LM (@LM_EM _ LM)}:
+  fairnessGpreS LM Σ.
+Proof. apply hGS. Defined. 
+
+(* TODO: get rid of it*)
+Global Instance LM_EM_fair `{LM: LiveModel heap_lang M}
+                `{hGS: @heapGS Σ LM (@LM_EM _ LM)}:
+  fairnessGS LM Σ.
+Proof. apply hGS. Defined.
+                                            
