fairness/examples/choose_nat/choose_nat.v
@@ -7,7 +7,7 @@ From iris.proofmode Require Import tactics.
 From trillium.prelude Require Export finitary quantifiers sigma classical_instances.
 From trillium.fairness Require Import fairness fair_termination fairness_finiteness.
 From trillium.program_logic Require Export weakestpre.
-From trillium.fairness.heap_lang Require Export lang lifting tactics proofmode simulation_adequacy.
+From trillium.fairness.heap_lang Require Export lang lifting tactics proofmode simulation_adequacy_lm.
 From trillium.fairness.heap_lang Require Import notation.
 
 Import derived_laws_later.bi.
