fairness/examples/yesno/yesno_adequacy.v
@@ -3,7 +3,7 @@ From iris.proofmode Require Import tactics.
 From trillium.program_logic Require Export weakestpre.
 From trillium.fairness Require Import fairness fair_termination fairness_finiteness.
 From trillium.prelude Require Export finitary quantifiers sigma classical_instances.
-From trillium.fairness.heap_lang Require Export lang tactics simulation_adequacy.
+From trillium.fairness.heap_lang Require Export lang tactics simulation_adequacy_lm.
 From trillium.fairness.heap_lang Require Import notation.
 
 From stdpp Require Import finite.
