fairness/heap_lang/simulation_adequacy_lm.v
@@ -1,0 +1,326 @@
+From iris.proofmode Require Import tactics.
+From trillium.fairness Require Import fuel fuel_termination fairness_finiteness resources.
+From trillium.fairness.heap_lang Require Export lang simulation_adequacy em_lm.
+
+Section adequacy.
+(* Local Hint Resolve tid_step_tp_length_heap: core. *)
+
+Theorem heap_lang_continued_simulation_fair_termination {FM : FairModel}
+        `{FairTerminatingModel FM} {LM:LiveModel heap_lang FM} ξ a1 r1 extr :
+  continued_simulation
+    (sim_rel_with_user LM ξ)
+    ({tr[trfirst extr]}) ({tr[initial_ls (LM := LM) a1 r1]}) →
+  extrace_fairly_terminating extr.
+Proof.
+  apply continued_simulation_fair_termination.
+  - intros ?? contra. inversion contra.
+    simplify_eq. inversion H2.
+  - by intros ex atr [[??]?].
+  - by intros ex atr [[??]?].
+Qed.
+
+Let rel_always_holds `{LM:LiveModel heap_lang M} `{hGS: @heapGS Σ LM (@LM_EM _ LM)}
+  s ξ e1 σ1 δ1 := 
+      rel_always_holds0 (fun etr atr => ξ etr (map_underlying_trace atr)) 
+        s (state_interp) (fun _ => 0%nat ↦M ∅) e1 σ1 δ1. 
+
+Lemma rel_always_holds_lift_LM `{LM: LiveModel heap_lang M} `{hGS: @heapGS Σ LM (@LM_EM _ LM)}
+  s e1 σ1 s1 ξ:
+  rel_always_holds s ξ e1 σ1 (initial_ls s1 0%nat) -∗
+  rel_always_holds0 (sim_rel_with_user LM ξ) s state_interp
+    (λ _, 0%nat ↦M ∅) e1 σ1 (initial_ls s1 0%nat).
+Proof.
+  iIntros "H".
+  iIntros (ex atr c Hvalex Hstartex Hstartatr Hendex Hcontr Hstuck Hequiv) "Hsi Hposts".
+  assert ( ∀ (ex' : finite_trace (cfg heap_lang) (olocale heap_lang)) (atr' : auxiliary_trace LM) (oζ : olocale heap_lang) (ℓ : mlabel LM),
+   trace_contract ex oζ ex' → trace_contract atr ℓ atr' → ξ ex' (map_underlying_trace atr')) as Hcontr'.
+  { intros ex' atr' oζ ℓ H1 H2. cut (sim_rel_with_user LM ξ ex' atr'); eauto. rewrite /sim_rel_with_user. intros [??]. done. }
+  iSpecialize ("H" $! ex atr c Hvalex Hstartex Hstartatr Hendex Hcontr' Hstuck Hequiv).
+  
+  unfold sim_rel_with_user.
+  iAssert (|={⊤}=> ⌜ξ ex (map_underlying_trace atr)⌝ ∗ state_interp ex atr ∗ posts_of c.1
+               ((λ _ : language.val heap_lang, 0%nat ↦M ∅)
+                :: ((λ '(tnew, e), fork_post (language.locale_of tnew e)) <$>
+                    prefixes_from [e1] (drop (length [e1]) c.1))))%I with "[Hsi H Hposts]" as "H".
+  { iApply fupd_plain_keep_l. iFrame. iIntros "[Hsi Hposts]".
+    iSpecialize ("H" with "Hsi Hposts").
+    by iApply fupd_plain_mask_empty. }
+  iMod "H" as "[H1 [Hsi Hposts]]".
+  destruct ex as [c'|ex' tid (e, σ)].
+  - (* We need to prove that the initial state satisfies the property *)
+    destruct atr as [δ|???]; last by inversion Hvalex. simpl.
+    have Heq1 := trace_singleton_ends_in_inv _ _ Hendex.
+    have Heq3 := trace_singleton_starts_in_inv _ _ Hstartex.
+    have Heq4 := trace_singleton_starts_in_inv _ _ Hstartex.
+    pose proof (trace_singleton_starts_in_inv _ _ Hstartatr). simpl.
+    simplify_eq.
+    iApply (fupd_mask_weaken ∅); first set_solver. iIntros "_ !>".
+    assert (∀ (ρ : fmrole M) (tid : nat),
+               ls_mapping (initial_ls (LM := LM) s1 0%nat) !! ρ = Some tid →
+               is_Some (([e1], σ1).1 !! tid)) as HA.
+    { simpl. intros ρ tid Hsome. apply lookup_gset_to_gmap_Some in Hsome as [??].
+      simplify_eq. by eexists _. }
+    iSplit; last done. iClear "H1".
+    iSplit; first done.
+    destruct (to_val e1) as [v1|] eqn:Heq.
+    + iSplit.
+      { iPureIntro. intros ρ tid Hinit.
+        simpl in *. apply lookup_gset_to_gmap_Some in Hinit as [_ <-].
+        rewrite /from_locale //. }
+      iIntros (tid e Hsome Hnoval ρ). destruct tid; last done.
+      simpl in Hsome. compute in Hsome. simplify_eq. simpl.
+      iAssert (0%nat ↦M ∅) with "[Hposts]" as "Hem".
+      { rewrite /= Heq /fmap /=. by iDestruct "Hposts" as "[??]". }
+      iDestruct "Hsi" as "(_&_&Hsi)".
+      iDestruct "Hsi" as "(%m&%FR'&Hfuela&Hmapa&HFR&%Hinvmap&%Hsmall&Hmodel&HfrFR)".
+      iDestruct (frag_mapping_same 0%nat m with "[Hmapa] Hem") as "%H"; [done| ].
+      iPureIntro. by eapply no_locale_empty.
+    + iSplit; iPureIntro.
+      { simpl. intros ρ tid Hsome. apply lookup_gset_to_gmap_Some in Hsome as [??].
+        simplify_eq. by eexists _. }
+      intros tid e Hsome Hval' ρ.
+      destruct tid as [|tid]; rewrite /from_locale /= in Hsome; by simplify_eq.
+  - (* We need to prove that that the property is preserved *)
+    destruct atr as [|atr' ℓ δ]; first by inversion Hvalex.
+    (* rewrite (trace_singleton_ends_in_inv _ _ Hendex); last exact unit. *)
+    specialize (Hcontr ex' atr' tid ℓ).
+    have H: trace_contract (trace_extend ex' tid (e, σ)) tid ex' by eexists.
+    have H': trace_contract (trace_extend atr' ℓ δ) ℓ atr' by eexists.
+    specialize (Hcontr H H') as Hvs. clear H H' Hcontr.
+    (* destruct Hvalex as (Hlm & Hlt & Hts). *)
+    have H: trace_ends_in ex' (trace_last ex') by eexists.
+    have H': trace_ends_in atr' (trace_last atr') by eexists.
+    iApply (fupd_mask_weaken ∅); first set_solver. iIntros "_ !>".
+    apply (trace_singleton_ends_in_inv (L := unit)) in Hendex.
+    simpl in *. simplify_eq.
+    iDestruct "Hsi" as "((%&%&%Htids)&_&Hsi)".
+    iDestruct "Hsi" as "(%m&%&Hfuela&Hmapa&?&%Hinvmap&%Hsmall&Hmodel&?)".
+    iSplit; [|done].
+    iSplit; [done|].
+    iSplit.
+    + iPureIntro. intros ρ tid' Hsome. simpl. unfold tids_smaller in Htids. eapply Htids. done.
+    + iIntros (tid' e' Hsome Hnoval ρ). simpl.
+      iAssert (tid' ↦M ∅) with "[Hposts]" as "H".
+      { destruct (to_val e') as [?|] eqn:Heq; last done.
+        iApply posts_of_empty_mapping => //.
+        apply from_locale_lookup =>//. }
+      iDestruct (frag_mapping_same tid' m with "Hmapa H") as "%Hlk".
+      { rewrite /auth_mapping_is. iPureIntro. by eapply no_locale_empty. }
+Qed.
+  
+
+Theorem strong_simulation_adequacy Σ `(LM:LiveModel heap_lang M)
+    `{hPre: @heapGpreS Σ LM (@LM_EM _ LM)} (s: stuckness) (e1 : expr) σ1 (s1: M)
+    (ξ : execution_trace heap_lang → finite_trace M (option $ fmrole M) →
+         Prop) :
+  rel_finitary (sim_rel_with_user LM ξ) →
+  (∀ `{hGS: @heapGS Σ LM (@LM_EM _ LM)}, 
+    ⊢ |={⊤}=>
+       ([∗ map] l ↦ v ∈ heap σ1, mapsto l (DfracOwn 1) v) ∗
+         LM_init_resource (initial_ls (LM := LM) s1 0%nat)
+       ={⊤}=∗
+       WP e1 @ s; locale_of [] e1; ⊤ {{ v, init_thread_post 0%nat }} ∗
+       rel_always_holds s ξ e1 σ1 (initial_ls (LM := LM) s1 0%nat)) ->
+  continued_simulation (sim_rel_with_user LM ξ) (trace_singleton ([e1], σ1)) (trace_singleton (initial_ls (LM := LM) s1 0%nat)).
+Proof.
+  intros Hfin WP_RAH.
+  eapply @strong_simulation_adequacy_general.
+  1-4: done. 
+  iIntros. iModIntro. 
+  iIntros "R". iMod (WP_RAH with "R") as ">[WP RAH]".
+  iModIntro. iSplitL "WP"; [by iFrame| ]. 
+  by iApply rel_always_holds_lift_LM. 
+Qed.
+
+Theorem simulation_adequacy Σ `(LM:LiveModel heap_lang M) `{hPre: @heapGpreS Σ LM (@LM_EM _ LM)} (s: stuckness) (e1 : expr) σ1 (s1: M):
+  (* The model has finite branching *)
+  rel_finitary (sim_rel LM) →
+  (* The initial configuration satisfies certain properties *)
+  (* A big implication, and we get back a Coq proposition *)
+  (* For any proper Aneris resources *)
+  (∀ `{hGS: @heapGS Σ LM (@LM_EM _ LM)},
+      ⊢ |={⊤}=>
+         LM_init_resource (initial_ls (LM := LM) s1 0%nat)
+        ={⊤}=∗ WP e1 @ s; 0%nat; ⊤ {{ v, init_thread_post 0%nat }}
+  ) ->
+  (* The coinductive pure coq proposition given by adequacy *)
+  @continued_simulation
+    heap_lang
+    LM
+    (sim_rel LM)
+    (trace_singleton ([e1], σ1))
+    (trace_singleton (initial_ls (LM := LM) s1 0%nat)).
+Proof.
+  intros Hne H.
+  assert (sim_rel LM = sim_rel_with_user LM (λ _ _, True)) as Heq.
+  { Require Import Coq.Logic.FunctionalExtensionality.
+    Require Import Coq.Logic.PropExtensionality.
+    do 2 (apply functional_extensionality_dep; intros ?).
+    apply propositional_extensionality.
+    unfold sim_rel_with_user. intuition. }
+
+  rewrite Heq.
+  apply (strong_simulation_adequacy Σ LM s) =>//.
+  { rewrite -Heq. done. }
+  iIntros (Hinv) "".
+  iPoseProof (H Hinv) as ">H". iModIntro. iIntros "[Hσ (Hm & Hfr & Hf)]". iSplitR "".
+  - iApply ("H" with "[Hm Hfr Hf]"). rewrite /LM_init_resource. iFrame. 
+  - iIntros "!>%%%?????????".
+    iApply (fupd_mask_weaken ∅); first set_solver. by iIntros "_ !>".
+Qed.
+
+Theorem simulation_adequacy_inftraces Σ `(LM: LiveModel heap_lang M)
+        `{hPre: @heapGpreS Σ LM (@LM_EM _ LM)}  (s: stuckness)
+        e1 σ1 (s1: M)
+        (iex : inf_execution_trace heap_lang)
+        (Hvex : valid_inf_exec (trace_singleton ([e1], σ1)) iex)
+  :
+  (* The model has finite branching *)
+  rel_finitary (sim_rel LM)  →
+  (∀ `{hGS: @heapGS Σ LM (@LM_EM _ LM)},
+      ⊢ |={⊤}=> LM_init_resource (initial_ls (LM := LM) s1 0%nat)
+         ={⊤}=∗ WP e1 @ s; 0%nat; ⊤ {{ v, init_thread_post 0%nat }}
+  ) ->
+  (* The coinductive pure coq proposition given by adequacy *)
+  exists iatr,
+  @valid_inf_system_trace _ LM
+    (@continued_simulation
+       heap_lang
+       LM
+       (sim_rel LM))
+    (trace_singleton ([e1], σ1))
+    (trace_singleton (initial_ls (LM := LM) s1 0%nat))
+    iex
+    iatr.
+Proof.
+  intros Hfin Hwp.
+  eexists.
+  eapply produced_inf_aux_trace_valid_inf.
+  Unshelve.
+  - econstructor.
+  - apply (simulation_adequacy Σ LM s) => //.
+  - done.
+Qed.
+
+Definition heap_lang_extrace : Type := extrace heap_lang.
+
+Theorem simulation_adequacy_traces Σ `(LM : LiveModel heap_lang M)
+  `{hPre: @heapGpreS Σ LM (@LM_EM _ LM)} (s: stuckness)
+        e1 (s1: M)
+        (extr : heap_lang_extrace)
+        (Hvex : extrace_valid extr)
+        (Hexfirst : (trfirst extr).1 = [e1])
+  :
+  (* The model has finite branching *)
+  rel_finitary (sim_rel LM) →
+  (∀ `{hGS: @heapGS Σ LM (@LM_EM _ LM)},
+      ⊢ |={⊤}=> LM_init_resource (initial_ls (LM := LM) s1 0%nat)
+        ={⊤}=∗ WP e1 @ s; 0%nat; ⊤ {{ v, init_thread_post 0%nat }}
+  ) ->
+  (* The coinductive pure coq proposition given by adequacy *)
+  ∃ (auxtr : auxtrace LM), exaux_traces_match extr auxtr.
+Proof.
+  intros Hfin Hwp.
+  have [iatr Hbig] : exists iatr,
+      @valid_inf_system_trace
+        heap_lang LM
+        (@continued_simulation
+           heap_lang
+           LM
+           (sim_rel LM))
+        (trace_singleton ([e1], (trfirst extr).2))
+        (trace_singleton (initial_ls (LM := LM) s1 0%nat))
+        (from_trace extr)
+        iatr.
+  { apply (simulation_adequacy_inftraces _ _ s); eauto.
+    eapply from_trace_preserves_validity; eauto; first econstructor.
+    simpl. destruct (trfirst extr) eqn:Heq.
+    simpl in Hexfirst. rewrite -Hexfirst Heq //. }
+  exists (to_trace (initial_ls (LM := LM) s1 0%nat) iatr).
+  eapply (valid_inf_system_trace_implies_traces_match (continued_simulation (sim_rel LM))); eauto.
+  - by intros ? ? [? ?]%continued_simulation_rel.
+  - by intros ? ? [? ?]%continued_simulation_rel.
+  - apply from_trace_spec. simpl. destruct (trfirst extr) eqn:Heq. simplify_eq. f_equal.
+    simpl in Hexfirst. rewrite -Hexfirst Heq //.
+  - apply to_trace_spec.
+Qed.
+
+
+Theorem simulation_adequacy_model_trace Σ `(LM : LiveModel heap_lang M)
+        `{hPre: @heapGpreS Σ LM (@LM_EM _ LM)} (s: stuckness)
+        e1 (s1: M)
+        (extr : heap_lang_extrace)
+        (Hvex : extrace_valid extr)
+        (Hexfirst : (trfirst extr).1 = [e1])
+  :
+  (* The model has finite branching *)
+  rel_finitary (sim_rel LM) →
+  (∀ `{hGS: @heapGS Σ LM (@LM_EM _ LM)},
+      ⊢ |={⊤}=> LM_init_resource (initial_ls (LM := LM) s1 0%nat) 
+               ={⊤}=∗ WP e1 @ s; 0%nat; ⊤ {{ v, init_thread_post 0%nat }}
+  ) ->
+  (* The coinductive pure coq proposition given by adequacy *)
+  ∃ (auxtr : auxtrace LM) mtr, exaux_traces_match extr auxtr ∧
+                               upto_stutter ls_under Ul auxtr mtr.
+Proof.
+  intros Hfb Hwp.
+  destruct (simulation_adequacy_traces
+              Σ _ _ e1 s1 extr Hvex Hexfirst Hfb Hwp) as [auxtr Hmatch].
+  assert (auxtrace_valid auxtr) as Hstutter.
+  { by eapply exaux_preserves_validity in Hmatch. }
+  destruct (can_destutter_auxtr auxtr) as [mtr Hupto] =>//.
+  eauto.
+Qed.
+  
+
+Theorem simulation_adequacy_terminate Σ `{LM:LiveModel heap_lang Mdl}
+        `{hPre: @heapGpreS Σ LM (@LM_EM _ LM)} (s: stuckness)
+        e1 (s1: Mdl)
+        (extr : heap_lang_extrace)
+        (Hexfirst : (trfirst extr).1 = [e1])
+  :
+  (∀ mtr: @mtrace Mdl, mtrace_fairly_terminating mtr) ->
+  (* The model has finite branching *)
+  rel_finitary (sim_rel LM) →
+  (∀ `{hGS: @heapGS Σ LM (@LM_EM _ LM)},
+      ⊢ |={⊤}=> LM_init_resource (initial_ls (LM := LM) s1 0%nat)
+                 ={⊤}=∗
+                 WP e1 @ s; 0%nat; ⊤ {{ v, init_thread_post 0%nat }}
+  ) ->
+  (* The coinductive pure coq proposition given by adequacy *)
+  extrace_fairly_terminating extr.
+Proof.  
+  intros Hterm Hfb Hwp Hvex Hfair.
+  destruct (simulation_adequacy_model_trace
+              Σ _ _ e1 s1 extr Hvex Hexfirst Hfb Hwp) as (auxtr&mtr&Hmatch&Hupto).
+  destruct (infinite_or_finite extr) as [Hinf|] =>//.
+  have Hfairaux := fairness_preserved extr auxtr Hinf Hmatch Hfair.
+  have Hvalaux := exaux_preserves_validity extr auxtr Hmatch.
+  have Hfairm := upto_stutter_fairness auxtr mtr Hupto Hfairaux.
+  have Hmtrvalid := upto_preserves_validity auxtr mtr Hupto Hvalaux.
+  have Htermtr := Hterm mtr Hmtrvalid Hfairm.
+  eapply exaux_preserves_termination =>//.
+  eapply upto_stutter_finiteness =>//.
+Qed.
+
+Theorem simulation_adequacy_terminate_ftm Σ `{FairTerminatingModel M}
+        `(LM : LiveModel heap_lang M)
+        `{hPre: @heapGpreS Σ LM (@LM_EM _ LM)} (s: stuckness)
+        e1 (s1: M)
+        (extr : heap_lang_extrace)
+        (Hexfirst : (trfirst extr).1 = [e1])
+  :
+  (* The model has finite branching *)
+  rel_finitary (sim_rel LM) →
+  (∀ `{hGS: @heapGS Σ LM (@LM_EM _ LM)},
+      ⊢ |={⊤}=> LM_init_resource (initial_ls (LM := LM) s1 0%nat) 
+               ={⊤}=∗ WP e1 @ s; 0%nat; ⊤ {{ v, init_thread_post 0%nat }}
+  ) ->
+  (* The coinductive pure coq proposition given by adequacy *)
+  extrace_fairly_terminating extr.
+Proof.
+  eapply simulation_adequacy_terminate =>//.
+  apply fair_terminating_traces_terminate.
+Qed.
+
+End adequacy.
